{
 "cells": [
  {
   "cell_type": "markdown",
   "metadata": {},
   "source": [
    "### $\\textbf{Task 1 Answers}$\n",
    "<br>"
   ]
  },
  {
   "cell_type": "markdown",
   "metadata": {},
   "source": [
    "$\\textbf{Question 1:}$ Demonstrate that the expected value $E[y]$ can be represented as $\\Sigma y \\cdot P(y) = n \\cdot p_i$.\n",
    "\n",
    "<b>Step 1:</b> Rewrite the expected value $E[y]$ using $P(y)$:\n",
    "\n",
    "$E[y] = \\Sigma_{y} \\, y \\cdot P(y)$\n",
    "\n",
    "<b>Step 2:</b> Substitute the provided joint probability distribution for $P(y)$:\n",
    "\n",
    "$E[y] = \\Sigma_{y} \\, y \\cdot (\\frac{n!}{y_1!y_2!y_3!...y_k!} \\cdot p_1^{y_1} p_2^{y_2} p_3^{y_3}....p_k^{y_k})$\n",
    "\n",
    "<b>Step 3:</b> Expand the summation:\n",
    "\n",
    "$E[y] = \\Sigma_{y} \\frac{n!}{y_1!y_2!y_3!...y_k!} \\cdot (y_1 \\cdot p_1) \\cdot (y_2 \\cdot p_2) \\cdot (y_3 \\cdot p_3) \\ldots (y_k \\cdot p_k)$\n",
    "\n",
    "<b>Step 4:</b> Rearrange terms:\n",
    "\n",
    "$E[y] =  \\frac{n!}{y_1!y_2!y_3!...y_k!} \\cdot \\Sigma_{y} (y_1 \\cdot p_1) \\cdot (y_2 \\cdot p_2) \\cdot (y_3 \\cdot p_3) \\ldots (y_k \\cdot p_k)$\n",
    "\n",
    "<b>Step 5:</b> Recognize that the sum is a product of sums:\n",
    "\n",
    "$E[y] =  \\frac{n!}{y_1!y_2!y_3!...y_k!} \\cdot  ( \\Sigma_{y_1} \\,y_1 \\cdot p_1) \\cdot (\\Sigma_{y_2} \\, y_2 \\cdot p_2) \\cdot ( \\Sigma_{y_3} \\, y_3 \\cdot p_3) \\ldots ( \\Sigma_{y_k} \\, y_k \\cdot p_k)$\n",
    "\n",
    "<b>Step 6:</b> Each individual sum represents the expected value of a binomial distribution with parameters $n$ and $p_i$:\n",
    "\n",
    "$E[Y_i] = n \\cdot p_i$\n",
    "\n",
    "<b>Step 7:</b> Substitute the expected values of each $Y_i$:\n",
    "\n",
    "$E[y] = \\frac{n!}{y_1!y_2!y_3!...y_k!} \\cdot (n \\cdot p_1) \\cdot (n \\cdot p_2) \\cdot (n \\cdot p_3) \\ldots  (n \\cdot p_k)$\n",
    "\n",
    "<b>Step 8:</b> Notice that $n!$ and $y_1!y_2!y_3!...y_k!$ cancel out:\n",
    "\n",
    "$E[y] = n \\cdot p_1 \\cdot n \\cdot p_2 \\cdot n \\cdot p_3 \\ldots n \\cdot p_k$\n",
    "\n",
    "Combining terms simplifies the expression, and recognizing that the coefficient $(y_1!y_2!y_3!...y_k!)$ simplifies to $n!$\n",
    "\n",
    "<b>Step 9:</b> Simplify:\n",
    "\n",
    "$E[y] = n  (p_1 \\cdot  p_2 \\cdot  p_3 \\ldots  p_k)$\n",
    "\n",
    "<b>Step 10:</b> Recall that $p_1 + p_2 + p_3 + \\ldots + p_k = 1$:\n",
    "\n",
    "$E[y] = n \\cdot 1$\n",
    "$E[y] = n \\cdot p_i$\n",
    "\n",
    "<b>Conclusion:</b> Therefore, the expected value $E[y]$ equals $\\Sigma y \\cdot P(y)$, which is equivalent to $n \\cdot p_i$."
   ]
  },
  {
   "cell_type": "markdown",
   "metadata": {},
   "source": [
    "$\\textbf{Question 2: }$ Given the data in the table above, if 500 adults are sampled  randomly, find the probability that the sample contains 100 person between 18 and 24, 200 between the ages of 25 and 34, and 200 between the ages of 45 and 64. What is the expected value for to obtain a person in the 65 and above?\n",
    "<br><br>\n",
    "\n",
    "<b>Given:</b>\n",
    "$n = 500$ (total number of adults sampled)\n",
    "$p_{65-100} = 0.16$ (probability of obtaining a person aged 65 and above)\n",
    "\n",
    "<br>\n",
    "\n",
    "<b>Step 1: </b>Apply the Formula \n",
    "The expected value $E[Y_{65+}]$ is given by:\n",
    "\n",
    "$ E[Y_{65+}] =  n \\cdot p_{65-100}$\n",
    "\n",
    "<b>Step 2: </b>Substitute Values\n",
    "\n",
    "$ E[Y_{65+}] = 500 \\cdot 0.16$\n",
    "$ E[Y_{65+}] = 80$\n",
    "\n",
    "<b>Conclusion: </b>Therefore, the expected value to obtain a person aged 65 and 100 given a sample size of 500 adults is 80."
   ]
  },
  {
   "cell_type": "markdown",
   "metadata": {},
   "source": [
    "### $\\textbf{Task 2 Answers}$\n",
    "<br>"
   ]
  },
  {
   "cell_type": "markdown",
   "metadata": {},
   "source": [
    "$\\textbf{Question 1: }$ From the following steps shown above, derive the probability distribution of the experiment.\n",
    "<br><br>\n",
    "\n",
    "The probability distribution of $Y$ follows the binomial distribution, which can be calculated using the binomial probability mass function:\n",
    "\n",
    "$P(Y = y) = \\binom{n}{y} \\cdot p^y \\cdot q^{n-y}$\n",
    "\n",
    "where:\n",
    "\n",
    "$P(Y = y)$ is the probabiltiy of observing $y$ successes in $n$ trials.\n",
    "$\\binom{n}{y}$ is the binomial coefficient , representing the number of ways to choose $y$ successes out of $n$ trials.\n",
    "$p^y$ represents the probability of having $y$ successes.\n",
    "$q^{n-y}$ represents the probability of having  $(n - y)$ failures.\n",
    "\n",
    "<br><br>"
   ]
  },
  {
   "cell_type": "markdown",
   "metadata": {},
   "source": [
    "$\\textbf{Question 2: }$ Show that the expectation of this probability distribution is $E[y] = \\Sigma y \\cdotp P(y) = np$.\n",
    "<br><br>\n",
    "\n",
    "\n",
    "<b>Step 1: </b>Define the Expectation\n",
    "\n",
    "$E[y] = \\Sigma_{y = 0}^n \\cdot P(y)$.\n",
    "\n",
    "<b>Step 2: </b>Utilize the Binomial Probability Mass Function\n",
    "\n",
    "$E[y] = \\Sigma_{y = 0}^n \\cdotp \\binom{n}{y} \\cdot p^y \\cdot q^{n-y}$.\n",
    "\n",
    "<b>Step 3: </b>Simplify the Expression\n",
    "\n",
    "Substitute $q$ with $1-p$ and rearrange terms.\n",
    "\n",
    "$E[y] = \\Sigma_{y = 0}^n \\frac{n!}{y!(n-y)!} \\cdot (p)^y \\cdot (1-p)^{(n-y)}$.\n",
    "\n",
    "<b>Step 4: </b>Factor Out Constants\n",
    "\n",
    "As $p$ is constant, it can be factored out of the summation.\n",
    "\n",
    "$E[y] = np \\, \\Sigma_{y = 0}^n \\frac{(n-1)!}{(y-1)!(n-y)!} \\cdot (p)^{(y-1)} \\cdot (1-p)^{(n-y)}$.\n",
    "\n",
    "<b>Step 5: </b>Rearrange the Terms\n",
    "\n",
    "$E[y] = np \\, \\Sigma_{y = 1}^n \\frac{(n-1)!}{(y-1)!(n-y)!} \\cdot (p)^{(y-1)} \\cdot (1-p)^{(n-y)}$.\n",
    " \n",
    "<b>Step 6: </b>Apply the Binomial Theorem\n",
    "\n",
    "Using the binomial theorem with positive integers $n$ and $k$, it states:\n",
    "\n",
    "$(x+y)^{n}= \\Sigma_{k=0}^{n}\\binom{n}{k} x^{k} y^{n-k}$ \n",
    "\n",
    " where: $\\binom{n}{k}$ denotes the binomial coefficient.\n",
    "\n",
    "$(p + q)^ {n -1} = \\Sigma_{k = 0}^{n-1} \\binom{n-1}{y} \\cdot (p)^{(k)} \\cdot (q)^{(n-1-k)}$\n",
    "\n",
    "Comparing terms to the binomial theorem, we find:\n",
    "\n",
    "$(p + q)^ {n-1} = \\Sigma_{y = 0}^{n} \\frac{(n-1)!}{(y)!(n-y)!} \\cdot (p)^{(y)} \\cdot (q)^{(n-y)}$\n",
    "\n",
    "<b>Step 7: </b>Simplify the expression\n",
    "\n",
    "Expanding $(p + (1-p))^{n-1}$ results in $1^{n-1}$, which equals 1. Thus, the sum becomes 1.\n",
    "\n",
    "This simplifies to:\n",
    "\n",
    "$E[y] = np \\cdot 1$, leading to the final simplification of $E[y] = np$.\n",
    "\n",
    "<b>Conclusion: </b>Hence, the expected value of a binomial distribution, $E[y] = np$, confirms that the mean equals the product of the number of trials and the probability of success.\n",
    "\n",
    "<br><br>"
   ]
  },
  {
   "cell_type": "markdown",
   "metadata": {},
   "source": [
    "$\\textbf{Question 3: }$ Experience has shown that 30% of all persons afflicted by a certain illness recover. A drug company has developed a new medication. Ten people with the illness were selected at random and received the medication; nine recovered shortly thereafter. Suppose that the medication was absolutely worthless. What is the probability that at least nine of ten receiving the medication will recover?\n",
    "<br><br>\n",
    "\n",
    "<b>Given:</b>\n",
    "\n",
    "-  Probability of success (recovery) $p = 0.30$\n",
    "-  Number of trials $n = 10$\n",
    "- Number of successes (recoveries) $y = 9$\n",
    "\n",
    "<b>Solution:</b>\n",
    "\n",
    "Using the binomial probability mass function:\n",
    "\n",
    "$P(Y \\geq 9) = P(Y = 9) + P(Y = 10)$\n",
    "\n",
    "$P(Y \\geq 9) = \\binom{10}{9} \\cdot (0.30)^9 \\cdot (1 - 0.30)^{10-9} + \\binom{10}{10} \\cdot (1 - 0.30)^{10-10}$\n",
    "\n",
    "$P(Y \\geq 9) = 10 \\cdot (0.30)^9 \\cdot (0.70)^1 + 1 \\cdot (0.30)^{10}  \\cdot (0.70)^0$\n",
    "\n",
    "$ P(Y \\geq 9) = 10 \\cdot (0.30)^9 \\cdot 0.70 + (0.30)^{10}$\n",
    "\n",
    "$ P(Y \\geq 9) = 0.000137781 + 0.0000059049$\n",
    "\n",
    "$ P (Y \\geq 9) \\approx 0.0001436869$ or $0.014 \\%$\n",
    "\n",
    "<b>Conclusion: </b>Therefore, the probability that at least nine of ten receiving the medication will recover is $0.014 \\%$.\n",
    "\n",
    "<br><br>"
   ]
  },
  {
   "cell_type": "markdown",
   "metadata": {},
   "source": [
    "$\\textbf{Question 4: }$ Suppose that a lot of 5000 electrical fuses contains 5% defectives. If a sample of 5 fuses is tested, find the probability of observing at least one defective.\n",
    "<br><br>\n",
    "\n",
    "<b>Given:</b>\n",
    "- Probability of success (a fuse being non-defective) $p = 0.95$\n",
    "- Number of trials $n = 5$\n",
    "\n",
    "<b>Solution:</b>\n",
    "\n",
    "$\\textbf{Solution:}$\n",
    "\n",
    "- To find the probability of observing at least one defective fuse, we can compute the complement of the probability of finding none defective.\n",
    "- So, $P(\\text{At least one defective}) = 1 - P(\\text{None defective})$.\n",
    "- This can also be expressed as $P(\\text{At least one defective}) = 1 - P(Y = 0)$.\n",
    "\n",
    "Using the binomial probability mass function:\n",
    "\n",
    "$P(Y=0) = \\binom {5}{0} \\cdot (0.05)^0 \\cdot (1 - 0.05)^{5-0}$\n",
    "\n",
    "$P(Y = 0) = (0.95)^5$\n",
    "\n",
    "$P(\\text{At least one defective}) = 1 - (0.95)^5$\n",
    "\n",
    "$P(\\text{At least one defective}) \\approx 1 - 0.7738$\n",
    "\n",
    "$P(\\text{At least one defective}) \\approx 0.2262$\n",
    "\n",
    "$\\textbf{Conclusion:}$ Hence, the probability of observing at least one defective fuse in a sample of 5 fuses is approximately $0.2262$ or $22.62\\%$."
   ]
  },
  {
   "cell_type": "markdown",
   "metadata": {},
   "source": [
    "### $\\textbf{Task 3 Solutions}$\n",
    "<br>"
   ]
  },
  {
   "cell_type": "markdown",
   "metadata": {},
   "source": [
    "$\\textbf{Question 1: }$ Find a general formula for the expected value of this distribution $p(y) = \\frac{\\lambda^y}{y!} e^{-\\lambda}$.\n",
    "<br><br>\n",
    "\n",
    "Given probability distribution: \n",
    "\n",
    "$p(y) = \\frac{\\lambda^y}{y!} e^{-\\lambda}$\n",
    "\n",
    "Expected value formula: \n",
    "\n",
    "$E[Y] = \\Sigma_{y=0} ^ \\infty \\, y \\cdot p(y)$\n",
    "\n",
    "<br>\n",
    "\n",
    "<b>Step 1: </b>Plug the Probability Distribution into the Expected Value Formula\n",
    "\n",
    "$E[Y] = \\Sigma_{y=0} ^ \\infty \\, y \\cdot \\frac{\\lambda^y}{y!} e^{-\\lambda}$\n",
    "\n",
    "<b>Step 2: </b>Factor out Constants\n",
    "\n",
    "$E[Y] = e^{-\\lambda} \\Sigma_{y=0} ^ \\infty \\, \\frac{\\lambda^y}{(y - 1)!} $\n",
    "\n",
    "<b>Step 3: </b>Since $y = 0$ renders $\\frac{\\lambda^y}{(y - 1)!}$ undefined, adjust the summation index to commence from $y = 1$.\n",
    "\n",
    "$E[Y] = e^{-\\lambda} \\Sigma_{y=1} ^ \\infty \\, \\frac{\\lambda^y}{(y - 1)!} $\n",
    "\n",
    "<b>Step 4: </b>Rewrite $\\frac{\\lambda^y}{(y - 1)!}$ as $\\frac{\\lambda^{(y-1)+ 1}}{(y - 1)!}$ \n",
    "\n",
    "$E[Y] = e^{-\\lambda} \\Sigma_{y=1} ^ \\infty \\,  \\frac{\\lambda^{(y-1)+ 1}}{(y - 1)!}$\n",
    "\n",
    "<b>Step 5: </b>Adjust the summation index to start from $y = 0$ to simplify the expression.\n",
    "\n",
    "$E[Y] = e^{-\\lambda} \\Sigma_{y=0} ^ \\infty \\,  \\frac{\\lambda^{y+1}}{y!}$\n",
    "\n",
    "<b>Step 6: </b>Factor out $\\lambda$\n",
    "\n",
    "$E[Y] = e^{-\\lambda} \\lambda \\Sigma_{y=0} ^ \\infty \\, \\frac {\\lambda^{y}}{y!}$\n",
    "\n",
    "<b>Step 7: </b>Recall that $e^{\\lambda} =  \\Sigma_{y=0} ^ \\infty \\, \\frac {\\lambda^{y}}{y!}$\n",
    "\n",
    "$E[Y] = e^{-\\lambda} \\lambda e^{\\lambda} $\n",
    "\n",
    "<b>Step 8: </b>Simplify: \n",
    "\n",
    "$E[Y] =  \\lambda$\n",
    "\n",
    "<b>Conclusion: </b>To conclude, the general expression for the expected value of the given distribution is $E[Y] =  \\lambda$\n",
    "\n",
    "<br><br>"
   ]
  },
  {
   "cell_type": "markdown",
   "metadata": {},
   "source": [
    "$\\textbf{Question 2: }$ A certain type of tree has seedlings randomly dispersed in a large area, with the mean density of seedlings being approximately five per square yard. If a forester randomly locates ten 1-square-yard sampling regions in the area, find the probability that none of the regions will contain seedlings.\n",
    "<br><br>\n",
    "\n",
    "<b>Given:</b>\n",
    "- $\\lambda = 5$\n",
    "\n",
    "<b>Solution: </b>\n",
    "\n",
    "Utilizing the Poisson distribution formula:\n",
    "\n",
    "$P(Y = y) = \\frac{\\lambda^y}{y!} e^{-\\lambda}$\n",
    "\n",
    "<br>\n",
    "\n",
    "For $y = 0$:\n",
    "\n",
    "$ P(Y = 0) = \\frac{5^0}{0!} e^{-5} $\n",
    "\n",
    "$ = e^{-5} $\n",
    "\n",
    "<br>\n",
    "\n",
    "Computing this probability:\n",
    "\n",
    "$P(Y = 0) \\approx e^{-5} $\n",
    "\n",
    "$\\approx 0.006737947$\n",
    "\n",
    "<b>Conclusion: </b>The probability of none of the regions containing seedlings is approximately $ 0.0067$ or $ 0.67\\%$."
   ]
  }
 ],
 "metadata": {
  "kernelspec": {
   "display_name": "Python 3 (ipykernel)",
   "language": "python",
   "name": "python3"
  },
  "language_info": {
   "codemirror_mode": {
    "name": "ipython",
    "version": 3
   },
   "file_extension": ".py",
   "mimetype": "text/x-python",
   "name": "python",
   "nbconvert_exporter": "python",
   "pygments_lexer": "ipython3",
   "version": "3.11.1"
  }
 },
 "nbformat": 4,
 "nbformat_minor": 4
}
