{
 "cells": [
  {
   "cell_type": "markdown",
   "id": "188d623d-79cb-4d7e-aaed-112bb84d8d33",
   "metadata": {},
   "source": [
    "\n",
    "$\\textbf{Assignment}$\n",
    "Instructions:\n",
    "- Use latex.\n",
    "- Write your latex in jupyter notebook.\n",
    "- Push your answer to your github account.\n",
    "- Deadline is 2 weeks before finals.\n",
    "- Fail to submit 2 weeks before finals is an automatic 5.0 for this assignment.\n",
    "- Each problem is 25 points.\n",
    "\n",
    "1. Recall the definition of a rational number, denoted as $\\mathbb{Q}$. Prove that the Euler's number $e = \\Sigma_{k=0}^\\infty \\frac{1}{k!} \\notin \\mathbb{Q}$. A factorial is defined as $k! = (k)(k-1)(k-2)(k-3)..., \\forall k \\in \\mathbb{Z}^+$, note that $0! = 1$. Furthermore, a sum notation $\\Sigma_{k=0}^\\infty k = 0+ 1 + 2 + 3 +....+...$\n",
    "\n",
    "## PROBLEM 1 SOLUTION:\n",
    "\n",
    "To prove that Euler's number is irrational, we can use a proof by contradiction. \n",
    "\n",
    "<b>Step 1:</b> We assume that $e$ is rational and can be expressed as a fraction of two integers $e = \\frac{p}{q}$ where $q \\neq 0$.\n",
    "\n",
    "<b>Step 2:</b> Power series\n",
    "\n",
    "$e^{x}$ = 1 + $x$ + $\\frac{x^{2}}{2!}$ + $\\frac{x^{3}}{3!}$ + ... = $\\sum_{n=0}^\\infty \\frac{x^{n}}{n!}$\n",
    "\n",
    "<b>Step 3:</b> Let x be -1\n",
    "\n",
    "$\\frac{1}{e}$ = $e^{-1}$ = 1 - 1 + $\\frac{1}{2!}$ + $\\frac{1}{3!}$ + ... =  $\\sum_{n=0}^\\infty \\frac{-1^{n}}{n!}$\n",
    "\n",
    "If $e \\in \\mathbb{Q}$, that means $\\frac{1}{e} = \\frac{q}{p} \\in \\mathbb{Q}$  for integers $p$ and $q$.\n",
    "\n",
    "$e^{-1}$ = $\\sum_{n=0}^p \\frac{-1^{n}}{n!}$ + $\\sum_{n=p+1}^\\infty \\frac{-1^{n}}{n!}$\n",
    "\n",
    "$\\frac{q}{p}$ - $\\sum_{n=0}^p \\frac{-1^{n}}{n!}$ = $\\sum_{n=p+1}^\\infty \\frac{-1^{n}}{n!}$\n",
    "\n",
    "<b>Step 4:</b> Multiply both sides by $-1^{p+1}p!$\n",
    "\n",
    "$-1^{p+1}q(p-1)! - (-1)^{p+1}(\\frac{p!}{2!} - \\frac{p!}{3!} + ... + \\frac{-1^{p}p!}{p!}) = \\frac{1}{p+1} - \\frac{1}{(p+1)(p+2)} + ...$\n",
    "\n",
    "We know that this series will converge to become smaller than the first term. We let the first term to be the upper bound and the lower bound to be the sum of the first two terms.\n",
    "\n",
    "Therefore $\\frac{1}{p+1} - \\frac{1}{(p+1)(p+2)} + ...$ must be between 0 and 1 since p > 1.\n",
    "\n",
    "We expected that each term are integers however this expression equated to a number between 0 and 1. This contradicts with our assumption that this expression is rational which proves that $e$ is irrational.\n",
    "\n",
    "## PROBLEM 2 SOLUTION:\n",
    "\n",
    "2. Prove Minkowski's Inequality for sums, $\\forall \\ p>1, (a_k, b_k)>0$:\n",
    "\\begin{gather}\n",
    "\\begin{bmatrix}\n",
    "\\Sigma_{k=1}^n |a_k + b_k|^p\n",
    "\\end{bmatrix}^\\frac{1}{p}\n",
    "\\leq\n",
    "\\begin{bmatrix}\n",
    "\\Sigma_{k=1}^n |a_k|^p\n",
    "\\end{bmatrix}^\\frac{1}{p}\n",
    "+\n",
    "\\begin{bmatrix}\n",
    "\\Sigma_{k=1}^n |b_k|^p\n",
    "\\end{bmatrix}^\\frac{1}{p}\n",
    "\\end{gather}\n",
    "\n",
    "<b>Step 1: </b> Let's start by considering Holder's inequality, which states:\n",
    "\n",
    "$\\sum_{k=1}^{n} |a_k b_k| \\leq \\left( \\sum_{k=1}^{n} |a_k|^p \\right)^{\\frac{1}{p}} \\left( \\sum_{k=1}^{n} |b_k|^q \\right)^{\\frac{1}{q}}$\n",
    "\n",
    "<b>Step 2: </b> We can define:\n",
    "\n",
    "$a_k = |x_k|^p $ , $ b_k = |y_k|^p $\n",
    "\n",
    "<b>Step 3: </b> Applying Holder's inequality with these definitions gives us:\n",
    "\n",
    "$ \\sum_{k=1}^{n} |x_k y_k|^p \\leq \\left( \\sum_{k=1}^{n} |x_k|^p \\right)^{\\frac{1}{p}} \\left( \\sum_{k=1}^{n} |y_k|^q \\right)^{\\frac{1}{q}} $\n",
    "\n",
    "<b>Step 4: </b> We take the $p$-th root of both sides:\n",
    "\n",
    "$ \\left( \\sum_{k=1}^{n} |x_k y_k|^p \\right)^{\\frac{1}{p}} \\leq \\left( \\sum_{k=1}^{n} |x_k|^p \\right)^{\\frac{1}{p}} \\left( \\sum_{k=1}^{n} |y_k|^p \\right)^{\\frac{1}{q}} \\ $\n",
    "\n",
    "<b>Step 5: </b> By exploiting the relationship between $p$ and $q$, we have:\n",
    "\n",
    "$ \\left( \\sum_{k=1}^{n} |x_k y_k|^p \\right)^{\\frac{1}{p}} \\leq \\left( \\sum_{k=1}^{n} |x_k|^p \\right)^{\\frac{1}{p}} \\left( \\sum_{k=1}^{n} |y_k|^p \\right)^{\\frac{p-1}{p}} \\ $\n",
    "\n",
    "<b>Step 6: </b> It's worth noting that: \n",
    "\n",
    "$ \\frac{p-1}{p} = 1 - \\frac{1}{p} \\ $\n",
    "\n",
    "<b>Step 7: </b> We apply Holder's inequality again to remove the $ \\frac{p-1}{p}\\ $ term:\n",
    "\n",
    "$ \\left( \\sum_{k=1}^{n} |y_k|^p \\right)^{\\frac{p-1}{p}} \\leq n^{\\frac{p-1}{p}} \\left( \\sum_{k=1}^{n} |y_k|^p \\right)^{\\frac{1}{p}} \\ $\n",
    "\n",
    "<b>Step 8: </b> Substituting this back into the inequality, we get:\n",
    "\n",
    "$ \\left( \\sum_{k=1}^{n} |x_k + y_k|^p \\right)^{\\frac{1}{p}} \\leq n^{\\frac{1}{p}} \\left( \\sum_{k=1}^{n} |x_k|^p \\right)^{\\frac{1}{p}} \\left( \\sum_{k=1}^{n} |y_k|^p \\right)^{\\frac{1}{p}} \\ $\n",
    "\n",
    "<b>Step 9: </b> The resulting expression represents the final form:\n",
    "\n",
    "$ \\left( \\sum_{k=1}^{n} |x_k + y_k|^p \\right)^{\\frac{1}{p}} \\leq n^{\\frac{1}{p}} \\left( \\sum_{k=1}^{n} |x_k|^p \\right)^{\\frac{1}{p}} \\left( \\sum_{k=1}^{n} |y_k|^p \\right)^{\\frac{1}{p}} \\ $\n",
    "   \n",
    "## PROBLEM 3 SOLUTION:\n",
    "\n",
    "3. Prove the triangle inequality $|x+y| \\leq |x| + |y|, \\forall (x,y) \\in \\mathbb{R}$\n",
    "\n",
    "<b>Step 1:</b> Understanding the concept of absolute value\n",
    "\n",
    "Definition:\n",
    "\\begin{gathered}\n",
    "{|x| = }\n",
    "\\begin{cases}\n",
    "x,&{x \\geq 0}\\\\ -x,&{x < 0}\n",
    "\\end{cases}\n",
    "\\end{gathered}\n",
    "\n",
    "Thus, we need to consider four scenarios:\n",
    "\\begin{gathered}\n",
    "\\textbf{Case 1: }{x \\geq 0, y \\geq 0} \\\\\n",
    "\\textbf{Case 2: }{x < 0, y < 0} \\\\\n",
    "\\textbf{Case 3: }{x \\geq 0, y < 0} \\\\\n",
    "\\textbf{Case 4: }{x < 0, y \\geq 0} \\\\\n",
    "\\end{gathered}\n",
    "\n",
    "$\\textbf{Case 1:} \\quad x \\geq 0, y \\geq 0$\n",
    "\n",
    "Let's equate $|x + y|$ to $x + y$, and $|x|$ to $x$, and $|y|$ to $y$.\n",
    "\n",
    "Substituting:\n",
    "\n",
    "\\begin{equation}\n",
    "|x + y| = x + y = |x| + |y|\n",
    "\\end{equation}\n",
    "$\\textbf{Case 2:} \\quad x < 0, y < 0$\n",
    "\n",
    "Let's equate $|x + y|$ to $-(x + y)$, and $|x|$ to $-x$, and $|y|$ to $-y$.\n",
    "\n",
    "Substituting:\n",
    "\n",
    "\\begin{equation}\n",
    "|x + y| = -(x + y) = -x - y = |x| + |y|\n",
    "\\end{equation}\n",
    "$\\textbf{Case 3:} \\quad x \\geq 0, y < 0$\n",
    "\n",
    "Let $|x| = x$, and $|y| = -y$.\n",
    "\n",
    "Substituting:\n",
    "\n",
    "\\begin{equation}\n",
    "|x + y| \\leq x - y\n",
    "\\end{equation}\n",
    "Considering two scenarios for $|x + y|$ since $x$ and $y$ have opposite signs:\n",
    "\n",
    "For $x + y \\geq 0$:\n",
    "\n",
    "\\begin{equation}\n",
    "x + y \\leq x - y \\implies y \\leq -y\n",
    "\\end{equation}\n",
    "For $x + y < 0$:\n",
    "\n",
    "\\begin{equation}\n",
    "-(x + y) \\leq x - y \\implies -x - y \\leq x - y \\implies -x \\leq x\n",
    "\\end{equation}\n",
    "$\\textbf{Case 4:} \\quad x < 0, y \\geq 0$\n",
    "\n",
    "Let $|x| = -x$, and $|y| = y$.\n",
    "\n",
    "Substituting:\n",
    "\n",
    "\\begin{equation}\n",
    "|x + y| \\leq -x + y\n",
    "\\end{equation}\n",
    "Solving for scenarios of $|x + y|$:\n",
    "\n",
    "For $x + y \\geq 0$:\n",
    "\n",
    "\\begin{equation}\n",
    "x + y \\leq -x + y \\implies x \\leq -x\n",
    "\\end{equation}\n",
    "For $x + y < 0$:\n",
    "\n",
    "\\begin{equation}\n",
    "-(x + y) \\leq -x + y \\implies -x - y \\leq -x + y \\implies -y \\leq y\n",
    "\\end{equation}\n",
    "\n",
    "\n",
    "## PROBLEM 4 SOLUTION:\n",
    "\n",
    "4. Prove Sedrakayan's Lemma $\\forall u_i, v_i \\in \\mathbb{R}^+$:\n",
    "\\begin{gather}\n",
    "\\frac{(\\Sigma_{i=1}^n u_i)^2}{\\Sigma_{i=1}^n v_i}\n",
    "\\leq\n",
    "\\Sigma_{i=1}^n \\frac{(u_i)^2}{v_i}\n",
    "\\end{gather}\n",
    "\n",
    "**Step 1: Applying Cauchy-Schwarz Inequality**\n",
    "\n",
    "We aim to prove Sedrakayan's Lemma, which asserts:\n",
    "\n",
    "Given positive real numbers $u_i$ and $v_i$ (where $i$ ranges from 1 to $n$), the following inequality holds:\n",
    "\\begin{gathered} \\frac{\\left(\\sum_{i=1}^n u_i\\right)^2}{\\sum_{i=1}^n v_i} \\leq \\sum_{i=1}^n \\frac{u_i^2}{v_i} \\end{gathered}\n",
    "\n",
    "To establish this, we leverage the Cauchy-Schwarz Inequality.\n",
    "\n",
    "**Step 2: Defining Vectors**\n",
    "\n",
    "Let's define two vectors:\n",
    "\n",
    "$\\mathbf{u} = (u_1, u_2, ..., u_n)$\n",
    "$\\mathbf{v} = (\\sqrt{v_1}, \\sqrt{v_2}, ..., \\sqrt{v_n})$\n",
    "\n",
    "**Step 3: Applying Cauchy-Schwarz Inequality**\n",
    "\n",
    "Now, we employ the Cauchy-Schwarz Inequality for inner products of vectors. This inequality posits that the square of the dot product of two vectors is less than or equal to the product of the squares of their magnitudes.\n",
    "\n",
    "For the sum of $u_i$, we have:\n",
    "\n",
    "$\\left(\\sum_{i=1}^n u_i\\right)^2 \\leq n \\left(\\sum_{i=1}^n u_i^2\\right)$\n",
    "For the sum of $\\sqrt{v_i}$, we have:\n",
    "\n",
    "$\\left(\\sum_{i=1}^n \\sqrt{v_i}\\right)^2 \\leq n \\left(\\sum_{i=1}^n v_i\\right)$\n",
    "\n",
    "**Step 4: Rearranging the Inequality**\n",
    "\n",
    "Rearranging the inequalities, we obtain:\n",
    "\n",
    "$\\frac{\\left(\\sum_{i=1}^n u_i\\right)^2}{\\sum_{i=1}^n v_i} \\leq \\frac{\\sum_{i=1}^n u_i^2}{\\sum_{i=1}^n v_i}$\n",
    "\n",
    "**Step 5: Final Form**\n",
    "\n",
    "Thus, we acknowledge the resulting expression as the final form:\n",
    "\\begin{gathered} \\frac{\\left(\\sum_{i=1}^n u_i\\right)^2}{\\sum_{i=1}^n v_i} \\leq \\frac{\\sum_{i=1}^n u_i^2}{\\sum_{i=1}^n v_i} \\end{gathered}\n"
   ]
  },
  {
   "cell_type": "markdown",
   "id": "fd17c1d3-e9fe-4b37-803e-8e11b24d7563",
   "metadata": {},
   "source": [
    "1. Consider the functions $f(x) = 2x+1$, $g(x)=2y-1$, $j(x) = |f(x)+g(x)|$, and $h(x) = j(x)^2$, show for the following inequality that:\n",
    "\\begin{gathered}\n",
    "\\sqrt{|f(x)|^2} \\geq \\sqrt{h(x)} - \\sqrt{|g(x)|^2}, \\forall (x,y) \\in \\mathbb{Z}^+\n",
    "\\end{gathered}\n"
   ]
  },
  {
   "cell_type": "markdown",
   "id": "aacef267-d99d-4258-90ab-8644ae669f1f",
   "metadata": {},
   "source": [
    "$\\textbf{Answer:}$\n",
    "\n",
    "Substitution:\n",
    "\n",
    "\\begin{gathered}\n",
    "\\sqrt{\\left|f\\left(x\\right)\\right|^2}\\ge \\sqrt{\\left|f\\left(x\\right)+g\\left(x\\right)\\right|^2}-\\sqrt{\\left|g\\left(x\\right)\\right|^2}\n",
    "\\end{gathered}\n",
    "\n",
    "Minkowski's Inequality for sums:\n",
    "\n",
    "\\begin{gathered}\n",
    "\\left|f\\left(x\\right)\\right|\\ge \\left|f\\left(x\\right)+g\\left(x\\right)\\right|-\\left|g\\left(x\\right)\\right|\n",
    "\\end{gathered}\n",
    "\n",
    "Transpose:\n",
    "\n",
    "\\begin{gathered}\n",
    "\\left|f\\left(x\\right)\\right|+\\left|g\\left(x\\right)\\right|\\ge \\left|f\\left(x\\right)+g\\left(x\\right)\\right|\n",
    "\\end{gathered}\n",
    "\n",
    "Rearrange to Triangle Inequality:\n",
    "\n",
    "\\begin{gathered}\n",
    "\\left|f\\left(x\\right)+g\\left(x\\right)\\right|\\le \\left|f\\left(x\\right)\\right|+\\left|g\\left(x\\right)\\right|\n",
    "\\end{gathered}\n",
    "\n",
    "Prove with the case: $f\\left(x\\right)>0$, and $g\\left(x\\right)>0$, Since $\\forall (x,y) \\in \\mathbb{Z}^+$\n",
    "\n",
    "Let $\\left|f\\left(x\\right)+g\\left(x\\right)\\right|=f\\left(x\\right)+g\\left(x\\right)$, and $|x|=x$, $|y|=y$\n",
    "\n",
    "Substitute:\n",
    "\\begin{gathered}\n",
    "\\left|f\\left(x\\right)+g\\left(x\\right)\\right|=f\\left(x\\right)+g\\left(x\\right)=\\left|f\\left(x\\right)\\right|+\\left|g\\left(x\\right)\\right|\n",
    "\\end{gathered}\n",
    "\n",
    "<br><br>"
   ]
  },
  {
   "cell_type": "markdown",
   "id": "72c04107-b462-4e6c-8ec3-b1f1df5fea6d",
   "metadata": {},
   "source": [
    "2. Prove Sedrakayan's Lemma if $u_i, v_i$ are square roots of an even integers:\n",
    "\\begin{gathered}\n",
    "\\frac{(\\Sigma_{i=1}^n u_i)^2}{\\Sigma_{i=1}^n v_i}\n",
    "\\leq\n",
    "\\Sigma_{i=1}^n \\frac{(u_i)^2}{v_i}\n",
    "\\end{gathered}"
   ]
  },
  {
   "cell_type": "markdown",
   "id": "5e5747bc-c1fb-466b-94d7-3d5444a5b96c",
   "metadata": {},
   "source": [
    "$\\textbf{Answer:}$\n",
    "\n",
    "Let $ u_i = \\sqrt{2a_i} $ and $ v_i = \\sqrt{2b_i} $, where $ a_i $ and $ b_i $ are positive integers. We need to show:\n",
    "\n",
    "$$\n",
    "\\frac{\\left( \\sum_{i=1}^n \\sqrt{2a_i} \\right)^2}{\\sum_{i=1}^n \\sqrt{2b_i}} \\leq \\sum_{i=1}^n \\frac{(2a_i)}{(2b_i)}\n",
    "$$\n",
    "\n",
    "Expand:\n",
    "\n",
    "$$\n",
    "\\frac{\\left( \\sum_{i=1}^n \\sqrt{2a_i} \\right)^2}{\\sum_{i=1}^n \\sqrt{2b_i}} = \\frac{\\left( \\sum_{i=1}^n \\sqrt{2a_i} \\right) \\left( \\sum_{i=1}^n \\sqrt{2a_i} \\right)}{\\sum_{i=1}^n \\sqrt{2b_i}}\n",
    "$$\n",
    "\n",
    "$$\n",
    "\\sum_{i=1}^n \\frac{(2a_i)}{(2b_i)} = \\sum_{i=1}^n \\frac{2a_i}{2b_i}\n",
    "$$\n",
    "\n",
    "Rewrite:\n",
    "\n",
    "$$\n",
    "\\frac{\\left( \\sum_{i=1}^n \\sqrt{2a_i} \\right)^2}{\\sum_{i=1}^n \\sqrt{2b_i}} \\leq \\sum_{i=1}^n \\frac{\\sqrt{2a_i}^2}{\\sqrt{2b_i}}\n",
    "$$\n",
    "\n",
    "Consider the following identity:\n",
    "\n",
    "$$\n",
    "\\left( \\sum_{i=1}^n x_i \\right)^2 = \\sum_{i=1}^n x_i^2 + 2 \\sum_{1 \\leq i < j \\leq n} x_i x_j\n",
    "$$\n",
    "\n",
    "Apply it to the numerator:\n",
    "\n",
    "$$\n",
    "\\frac{\\left( \\sum_{i=1}^n \\sqrt{2a_i} \\right)^2}{\\sum_{i=1}^n \\sqrt{2b_i}} = \\frac{\\sum_{i=1}^n (2a_i) + 2 \\sum_{1 \\leq i < j \\leq n} \\sqrt{2a_i} \\sqrt{2a_j}}{\\sum_{i=1}^n \\sqrt{2b_i}}\n",
    "$$\n",
    "\n",
    "\n",
    "Since $2a_i$ and $2b_i$ are even integers, $2 \\sum_{1 \\leq i < j \\leq n} \\sqrt{2a_i} \\sqrt{2a_j}$ is also even:\n",
    "\n",
    "$$\n",
    "\\frac{\\sum_{i=1}^n (2a_i)}{\\sum_{i=1}^n \\sqrt{2b_i}} + \\frac{2 \\sum_{1 \\leq i < j \\leq n} \\sqrt{2a_i} \\sqrt{2a_j}}{\\sum_{i=1}^n \\sqrt{2b_i}} \\leq \\sum_{i=1}^n \\frac{(2a_i)}{\\sqrt{2b_i}}\n",
    "$$\n",
    "\n",
    "Simplify:\n",
    "\n",
    "$$\n",
    "\\frac{\\sum_{i=1}^n (2a_i)}{\\sum_{i=1}^n \\sqrt{2b_i}} \\leq \\sum_{i=1}^n \\frac{(2a_i)}{\\sqrt{2b_i}}\n",
    "$$\n",
    "\n",
    "Given that both expressions in the inequality are non-negative and the terms in the numerator of the left side correspond to those in the denominator of the right side, the inequality is confirmed.\n",
    "\n",
    "Thus, Sedrakayan's Lemma is proven for $u_i$ and $v_i$ being square roots of even integers."
   ]
  },
  {
   "cell_type": "code",
   "execution_count": null,
   "id": "e5e14665-a468-4d56-87c2-91bc936bd58e",
   "metadata": {},
   "outputs": [],
   "source": []
  }
 ],
 "metadata": {
  "kernelspec": {
   "display_name": "Python 3 (ipykernel)",
   "language": "python",
   "name": "python3"
  },
  "language_info": {
   "codemirror_mode": {
    "name": "ipython",
    "version": 3
   },
   "file_extension": ".py",
   "mimetype": "text/x-python",
   "name": "python",
   "nbconvert_exporter": "python",
   "pygments_lexer": "ipython3",
   "version": "3.11.1"
  }
 },
 "nbformat": 4,
 "nbformat_minor": 5
}
